examples/low-level/crypto/Crypto.AEAD.Invariant.fst
@@ -50,6 +50,7 @@ type rw = | Reader | Writer
 noeq type state (i:id) (rw:rw) =
   | State:
       #log_region: rgn -> // this is the *writer* region; the reader allocates nothing
+      // the log should exist only when prf i
       log: HS.ref (Seq.seq (entry i)) {HS.frameOf log == log_region} ->
       // Was PRF(prf.rgn) == region. Do readers use its own PRF state?
       prf: PRF.state i {PRF(prf.rgn) == log_region} (* including its key *) ->
